Modules/TypeSystem/OmegaGroupoidCat.v
@@ -1,0 +1,135 @@
+
+(* an omega groupoid is an omega cat *)
+Require Import ssreflect ssrfun ssrbool .
+
+From Modules Require Import libhomot untypeduippackrl buildrlhp lib gensyntax brunerietype gtypeext omegagroupoids omegacategories.
+Require Import Coq.Logic.JMeq.
+Set Bullet Behavior "Strict Subproofs".
+
+Set Implicit Arguments.
+Unset Strict Implicit.
+Unset Printing Implicit Defensive.
+
+Local Notation "⟦ X ⟧V" := (dTm (w_va X)).
+
+Local Notation SB := (brunerietype.syntax).
+Local Notation SC := (ericsam.syntax).
+
+Module Syn := defsyntax.
+Local Notation "'WC' S" := (@Syn.WC _ S) (at level 0).
+Local Notation "'WTy' S" := (@Syn.WTy _ S)(at level 0).
+Local Notation "'Wtm' S":= (@Syn.Wtm _ S)(at level 0).
+Local Notation "'WS' S":= (@Syn.WS _ S)(at level 0).
+Local Notation "'SC_WVar' S":= (ericsam.WVar S)(at level 0).
+Local Notation "'SB_WVar' S":= (brunerietype.WVar S)(at level 0).
+(*
+Local Notation WTy := (@Syn.WTy _).
+Local Notation Wtm := (@Syn.Wtm _).
+Local Notation WS := (@Syn.WS _).
+Local Notation SC_WVar := (ericsam.WVar).
+Local Notation SB_WVar := (brunerietype.WVar).
+*)
+
+(*
+La syntaxe bien typée d'eric sam s'inject dans la syntaxe bien typée de Brunerie
+ *)
+
+Fixpoint wCB_C (Γ : Con) (wΓ : WC SC Γ) : WC SB Γ
+with wCB_T Γ A (wA : WTy SC Γ A) : WTy SB Γ A
+with wCB_Tm Γ A t (wt : Wtm SC Γ A t) : Wtm SB Γ A t
+with wCB_V Γ A x (wx : SC_WVar Γ A x) : SB_WVar Γ A x
+with wCB_S Γ Δ σ (wσ : WS SC Γ Δ σ) : WS SB Γ Δ σ.
+  - destruct wΓ.
+    + constructor.
+    + constructor.
+      * apply:wCB_C => //.
+      * apply:wCB_T => //.
+      * constructor.
+        apply:wCB_V => //.
+  - destruct wA.
+    + constructor.
+      apply:wCB_C => //.
+    + constructor.
+      * apply:wCB_T => //.
+      * apply:wCB_Tm => //.
+      * apply:wCB_Tm => //.
+  - destruct wt.
+    + constructor.
+      by apply:wCB_V => //.
+    + constructor.
+      * apply:wCB_C => //.
+      * apply:wCB_T => //.
+      * apply:wCB_S => //.
+    + rewrite -/((ar  A t u).[σ]T).
+      constructor.
+      * apply:wCB_C => //.
+      * constructor.
+        -- apply:wCB_T => //.
+        -- apply:wCB_Tm => //.
+        -- apply:wCB_Tm => //.
+      * apply:wCB_S => //.
+ - destruct wx.
+   + constructor.
+   + constructor.
+     * apply:wCB_V => //.
+     * apply:wCB_Tm => //.
+   + constructor.
+     apply:wCB_Tm => //.
+   + constructor.
+     apply:wCB_Tm => //.
+ - destruct wσ.
+   + constructor.
+     apply:wCB_Tm => //.
+   + constructor.
+      * apply:wCB_S => //.
+      * apply:wCB_T => //.
+      * apply:wCB_Tm => //.
+      * apply:wCB_Tm => //.
+      * apply:wCB_Tm => //.
+Defined.
+
+Section GroupoidToCat.
+  Context (d : @Decl _ SB).
+
+  Definition d' : @Decl _ SC :=
+    {|
+      dC := fun Γ  (wΓ : Syn.WC Γ) => ⟦ wCB_C wΓ ⟧C;
+      dTy := fun (Γ : Con) (A : Ty) (wΓ : Syn.WC Γ) (wA : Γ ⊢ A) => ⟦ wCB_T wA ⟧T;
+      dTm := fun (Γ : Con) (A : Ty) (t : Tm) (wΓ : Syn.WC Γ) (wt : Γ ⊢ t : A) (wA : Γ ⊢ A) =>
+               ⟦ wCB_Tm wt ⟧t (wCB_T wA);
+      dS := fun (Γ Δ : Con) (σ : sub) (wσ : ericsam.WS Γ Δ σ) (wΓ : ericsam.WC Γ) (wΔ : ericsam.WC Δ) =>
+              ⟦ wCB_S wσ ⟧S (wCB_C wΓ)(wCB_C wΔ) |}.
+
+  Import omegagroupoids.
+  Lemma isGroupoid_isCat (G : GType)  (gr : isOmegaGroupoid G d) : isOmegaCategory G d'.
+    constructor.
+    - by apply:dC_astar.
+    - intros.
+      apply:(dC_ext gr).
+    - intros.
+      apply:(dT_star gr).
+    - intros.
+      apply:(dT_ar gr).
+    - intros.
+      simpl.
+      apply:JMeq_trans; last by apply:(sb_dTm gr).
+      match goal with
+        [ |- ⟦ ?w1 ⟧t ?w2 γ ≅ ⟦ ?w3 ⟧t ?w4 γ ] =>
+        rewrite (WTm_hp w1 w3) (WTy_hp w2 w4)
+      end.
+      easy.
+    - apply:(dTm_vstar gr).
+    - intros; apply:(dTm_v1 gr).
+      eassumption.
+    - intros; apply:(dTm_v0 gr) => //.
+    - intros; apply:(dTm_vwk gr) => //.
+      eassumption.
+    - intros;apply:(dS_to_star gr) => //.
+    - intros;apply:(dS_to_ext gr) => //.
+      exact:H.
+      exact:H0.
+      exact:H1.
+  Qed.
+
+End GroupoidToCat.
+
