Modules/TypeSystem/gensyntax.v
@@ -1,0 +1,222 @@
+From Modules Require Import defsyntax.
+From Modules Require Export defsyntax.
+
+Set Implicit Arguments.
+Unset Strict Implicit.
+Unset Printing Implicit Defensive.
+
+Inductive Tm : Type :=
+  | va (x:Var)
+          (* Coh Γ A σ  *)
+  | coh : Con -> Ty -> sub -> Tm
+with Ty : Type :=
+  | star
+  | ar : Ty -> Tm -> Tm -> Ty
+with  Con : Type :=
+      | astar
+          (* Γ A, u tq Γ ⊢ u : A *)
+      | ext : Con -> Ty -> Tm -> Con
+with sub : Type :=
+       | to_star : Tm -> sub
+       | to_ext : sub -> Tm -> Tm -> sub
+with Var : Type :=
+  | vstar
+  (* toutes ces variables sont dans des contextes étendues *)
+  | vwk (v : Var)
+  | v0 
+  | v1 .
+
+Module S := defsyntax.
+
+Instance preSyntax : PreSyntax := {| S.Con := Con ;  S.Ty := Ty ; S.Tm := Tm ; S.sub := sub |}.
+
+
+(*
+Reserved Notation "Gamma ⊢ A : B"
+  (at level 68, A at level 99, no associativity,
+   format "Gamma  ⊢  A  :  B").
+Reserved Notation "Gamma ⊢ A"
+  (at level 68, A at level 99, no associativity,
+   format "Gamma  ⊢  A").
+
+Reserved Notation "Gamma ⊢ A ⇒ B"
+  (at level 68, A at level 99, no associativity,
+   format "Gamma  ⊢  A  ⇒  B").
+
+Reserved Notation "Gamma ⊢_v A : B"
+  (at level 68, A at level 99, no associativity,
+   format "Gamma  ⊢_v  A  :  B").
+
+Notation "Gamma ⊢ A" := (WTy Gamma A)  : wf_scope.
+Notation "Gamma ⊢ s : A" := (Wtm Gamma A s) : wf_scope.
+Notation "Gamma ⊢  s  ⇒ Delta" :=
+  (WS Gamma Delta s)
+    : wf_scope.
+
+Open Scope wf_scope.
+
+(* Reserved Notation "sigma ∘ tau"  (at level 56, left associativity). *)
+
+Reserved Notation "s .[ sigma ]T" (at level 2, sigma at level 200, left associativity,
+   format "s .[ sigma ]T" ).
+Reserved Notation "s .[ sigma ]oT" (at level 2, sigma at level 200, left associativity,
+   format "s .[ sigma ]oT" ).
+
+Reserved Notation "s .[ sigma ]wT" (at level 2, sigma at level 200, left associativity,
+   format "s .[ sigma ]wT" ).
+
+Reserved Notation "s .[ sigma ]t" (at level 2, sigma at level 200, left associativity,
+   format "s .[ sigma ]t" ).
+
+Reserved Notation "s .[ sigma ]V" (at level 2, sigma at level 200, left associativity,
+   format "s .[ sigma ]V" ).
+
+
+*)
+
+Fixpoint sub_Var (σ : sub) (x : Var) : Tm :=
+   match σ,x with
+     to_star t, vstar => t
+   | to_ext σ a f, vwk x => x .[ σ ]V
+   | to_ext σ a f, v0 => f
+   | to_ext σ a f, v1 => a
+   | _,_ => va vstar (* dummy *)
+   end
+where "s .[ sigma ]V" := (sub_Var sigma s) : subst_scope.
+
+
+Fixpoint sub_Tm (σ : sub) (t : Tm) : Tm :=
+  match t with
+  | va x => x .[ σ ]V
+          (* Coh Γ A σ  *)
+  | coh Γ A δ => coh Γ A (compS δ σ)
+  end
+    (*
+Γ ⊢ σ : Δ
+E ⊢ δ : Γ
+E ⊢ σ ∘ δ : Δ
+     *)
+with compS (σ : sub) (δ : sub) : sub :=
+       match σ with
+         | to_star t => to_star (t .[ δ ]t)
+         (* Γ ⊢ σ' : Δ' *)
+         (* E ⊢ σ ∘ δ : Δ *)
+         (* E ⊢ (σ ∘ δ)' : Δ' *)
+         | to_ext σ a f => to_ext (compS σ δ) (a .[ δ ]t) (f .[ δ ]t)
+       end
+where "s .[ sigma ]t" := (sub_Tm sigma s) : subst_scope.
+Notation "sigma ∘ delta"  :=(compS sigma delta)(at level 40, left associativity) : subst_scope.
+
+
+(* Γ ⊢ idS : Γ *)
+Fixpoint idS (Γ : Con) : sub :=
+  match Γ with
+    astar => to_star (va vstar)
+  | ext Γ A u => to_ext (idS Γ) (va v1) (va v0)
+  end.
+
+
+Fixpoint wkt (t : Tm) : Tm :=
+  match t with
+    va x => va (vwk x)
+  | coh Γ A σ => coh Γ A (wkS σ)
+  (* | coh_ar Γ A t u σ => coh_ar Γ A t u (wkS σ) *)
+  end
+with wkS (σ : sub) : sub :=
+  match σ with
+  | to_star t => to_star (wkt t)
+  | to_ext σ a f => to_ext (wkS σ) (wkt a) (wkt f)
+  end.
+
+Fixpoint wkT (A : Ty) : Ty :=
+  match A with
+    star => star
+  | ar A t u => ar (wkT A) (wkt t) (wkt u)
+  end.
+
+
+Open Scope subst_scope.
+
+
+Fixpoint sub_Ty (σ : sub) (A : Ty) : Ty :=
+  match A with
+    star => star
+  | ar A t u => ar (A .[ σ ]T) (t .[ σ ]t) (u .[ σ ]t)
+  end
+    where "s .[ sigma ]T" := (sub_Ty sigma s) : subst_scope.
+
+
+(* Definition sub_oTy (σ : sub) (A : option Ty) : option Ty := *)
+(*   if A is Some A then Some (A .[ σ ]T) else None. *)
+
+(* Notation "s .[ σ ]oT" := (sub_oTy σ s) : subst_scope. *)
+
+  
+(*
+Fixpoint beq_var ( x y : Var) : bool :=
+  match x,y with
+    vstar,vstar => true
+  | vwk v, vwk v' => beq_var v v'
+  | v0,v0 => true
+  | v1, v1 => true
+  | _,_ => false
+  end.
+  
+Fixpoint beq_tm (x y : Tm) : bool :=
+        (match x,y with
+       | va x, va x' => beq_var x x'
+       | coh Γ A σ, coh Γ' A' σ' => [ && beq_Con Γ Γ' , beq_Ty A A' & beq_sub σ σ' ]
+       | _,_ => false
+         end)
+with beq_Ty (x y : Ty) :=
+       (
+       match x,y with
+       | star, star => true
+       | ar A t u, ar A' t' u' =>
+         [ && beq_Ty A A' , beq_tm t t' & beq_tm u u' ]
+       (* | none,none => true *)
+       | _,_ => false
+
+       end)
+with beq_Con (x y : Con) :   bool :=
+      (match x , y with
+  | astar, astar => true
+  | ext Γ A u, ext Γ' A' u' => [ && beq_Con Γ Γ' , beq_Ty A A' & beq_tm u u' ]
+  | _,_ => false
+     end)
+with beq_sub (x y : sub) :   bool :=
+  (match x , y with
+      | to_star t, to_star t' => beq_tm t t'
+      | to_ext σ a f, to_ext σ' a' f' => [ && beq_sub σ σ' , beq_tm a a' & beq_tm f f']
+        | _,_ => false
+        end).
+
+*)
+(*
+Definition Var_eqP : Equality.axiom beq_var.
+Admitted.
+Definition tm_eqP : Equality.axiom beq_tm.
+Admitted.
+Definition Ty_eqP : Equality.axiom beq_Ty.
+Admitted.
+Definition sub_eqP : Equality.axiom beq_sub.
+Admitted.
+Definition Con_eqP : Equality.axiom beq_Con.
+Admitted.
+
+Canonical var_eqMixin := EqMixin Var_eqP.
+Canonical var_eqType := Eval hnf in EqType Var var_eqMixin.
+
+Canonical tm_eqMixin := EqMixin tm_eqP.
+Canonical tm_eqType := Eval hnf in EqType Tm tm_eqMixin.
+
+Canonical Ty_eqMixin := EqMixin Ty_eqP.
+Canonical Ty_eqType := Eval hnf in EqType Ty Ty_eqMixin.
+
+Canonical sub_eqMixin := EqMixin sub_eqP.
+Canonical sub_eqType := Eval hnf in EqType sub sub_eqMixin.
+
+Canonical Con_eqMixin := EqMixin Con_eqP.
+Canonical Con_eqType := Eval hnf in EqType Con Con_eqMixin.
+
+*)
