Modules/TypeSystem/gtypeext.v
@@ -1,0 +1,44 @@
+Require Import ssreflect ssrfun ssrbool .
+
+From Modules Require Import defsyntax libhomot lib.
+Require Import Coq.Logic.JMeq.
+Set Bullet Behavior "Strict Subproofs".
+
+Set Implicit Arguments.
+Unset Strict Implicit.
+Unset Printing Implicit Defensive.
+
+CoInductive GType :=
+  Gtyp { ob :> Type ;
+         hom :> ob -> ob -> GType }.
+
+Class Decl {P : PreSyntax} {S : Syntax} :=
+  { dC : forall Γ, WC Γ -> Type;
+    dTy : forall Γ A (wΓ : WC Γ)(wA: Γ ⊢ A), dC wΓ -> GType ;
+    dTm : forall Γ A t (wΓ : WC Γ)(wt : Γ ⊢ t : A)(wA: Γ ⊢ A)(γ : dC wΓ) ,
+            dTy wA γ;
+    dS : forall Γ Δ σ (wσ: Γ ⊢ σ ⇒ Δ)(wΓ : WC Γ)(wΔ : WC Δ) (γ : dC wΓ),
+            dC wΔ
+  }.
+
+Definition extΣ (Γ : Type) (A : Γ -> Type) (B : forall γ (a : A γ), Type) :=
+  { δ : { γ : Γ & A γ} & B (δ..1) δ..2}.
+
+Definition extΣ_G (Γ : Type) (A : Γ -> GType) (u : forall γ, A γ) :=
+  { δ : { γ : Γ & A γ} & hom δ..2 (u δ..1) }.
+
+Notation "⟦ X ⟧C" := (dC X).
+Notation "⟦ X ⟧T" := (dTy X).
+Notation "⟦ X ⟧t" := (dTm X).
+Notation "⟦ X ⟧S" := (dS X).
+
+CoFixpoint G_of_T (T : Type) : GType.
+  unshelve econstructor.
+  - exact:T.
+  - move => a b.
+    apply:G_of_T.
+    exact: (a =h b).
+Defined.
+(* Notation "∣ X ∣" := (ob X). *)
+
+
