Modules/TypeSystem/defsyntax.v
@@ -1,0 +1,63 @@
+
+Set Implicit Arguments.
+Unset Strict Implicit.
+Unset Printing Implicit Defensive.
+
+Class PreSyntax  :=
+  {
+    Con : Type;
+    Ty : Type;
+    Tm : Type;
+    sub : Type;
+    }.
+Class Syntax {S : PreSyntax} :=
+  {
+    WC : Con -> Type;
+    WTy : Con -> Ty -> Type;
+    Wtm : Con -> Ty -> Tm -> Type;
+    WS : Con -> Con -> sub -> Type }.
+Reserved Notation "Gamma ⊢"
+  (at level 68,  no associativity,
+   format "Gamma  ⊢ ").
+
+Reserved Notation "Gamma ⊢ A : B"
+  (at level 68, A at level 99, no associativity,
+   format "Gamma  ⊢  A  :  B").
+Reserved Notation "Gamma ⊢ A"
+  (at level 68, A at level 99, no associativity,
+   format "Gamma  ⊢  A").
+
+Reserved Notation "Gamma ⊢ A ⇒ B"
+  (at level 68, A at level 99, no associativity,
+   format "Gamma  ⊢  A  ⇒  B").
+
+Reserved Notation "Gamma ⊢_v A : B"
+  (at level 68, A at level 99, no associativity,
+   format "Gamma  ⊢_v  A  :  B").
+
+Notation "Gamma ⊢ " := (WC Gamma )  : wf_scope.
+Notation "Gamma ⊢ A" := (WTy Gamma A)  : wf_scope.
+Notation "Gamma ⊢ s : A" := (Wtm Gamma A s) : wf_scope.
+Notation "Gamma ⊢  s  ⇒ Delta" :=
+  (WS Gamma Delta s)
+    : wf_scope.
+
+Open Scope wf_scope.
+
+(* Reserved Notation "sigma ∘ tau"  (at level 56, left associativity). *)
+
+Reserved Notation "s .[ sigma ]T" (at level 2, sigma at level 200, left associativity,
+   format "s .[ sigma ]T" ).
+Reserved Notation "s .[ sigma ]oT" (at level 2, sigma at level 200, left associativity,
+   format "s .[ sigma ]oT" ).
+
+Reserved Notation "s .[ sigma ]wT" (at level 2, sigma at level 200, left associativity,
+   format "s .[ sigma ]wT" ).
+
+Reserved Notation "s .[ sigma ]t" (at level 2, sigma at level 200, left associativity,
+   format "s .[ sigma ]t" ).
+
+Reserved Notation "s .[ sigma ]V" (at level 2, sigma at level 200, left associativity,
+   format "s .[ sigma ]V" ).
+
+Reserved Notation "sigma ∘ delta"  (at level 40, left associativity).
